Revert "Merge branch 'robbert/sprop' into 'master'"
This reverts merge request !309

theories/coPset.v
@@ -68,7 +68,7 @@ Proof.
   assert (r = coPLeaf b) as -> by (apply IHr; try apply (λ p, Ht (p~1)); eauto).
   by destruct b.
 Qed.
-Lemma coPset_wf_eq t1 t2 :
+Lemma coPset_eq t1 t2 :
   (∀ p, e_of p t1 = e_of p t2) → coPset_wf t1 → coPset_wf t2 → t1 = t2.
 Proof.
   revert t2.
@@ -115,26 +115,15 @@ Fixpoint coPset_opp_raw (t : coPset_raw) : coPset_raw :=
   | coPNode b l r => coPNode' (negb b) (coPset_opp_raw l) (coPset_opp_raw r)
   end.
 
-Lemma coPset_singleton_wf p : SIs_true (coPset_wf (coPset_singleton_raw p)).
-Proof. apply SIs_true_intro. induction p; simpl; eauto. Qed.
-Lemma coPset_union_wf t1 t2 :
-  SIs_true (coPset_wf t1) → SIs_true (coPset_wf t2) →
-  SIs_true (coPset_wf (t1 ∪ t2)).
-Proof.
-  intros Hwf1%SIs_true_elim Hwf2%SIs_true_elim.
-  apply SIs_true_intro. revert Hwf1 Hwf2.
-  revert t2; induction t1 as [[]|[]]; intros [[]|[] ??]; simpl; eauto.
-Qed.
+Lemma coPset_singleton_wf p : coPset_wf (coPset_singleton_raw p).
+Proof. induction p; simpl; eauto. Qed.
+Lemma coPset_union_wf t1 t2 : coPset_wf t1 → coPset_wf t2 → coPset_wf (t1 ∪ t2).
+Proof. revert t2; induction t1 as [[]|[]]; intros [[]|[] ??]; simpl; eauto. Qed.
 Lemma coPset_intersection_wf t1 t2 :
-  SIs_true (coPset_wf t1) → SIs_true (coPset_wf t2) →
-  SIs_true (coPset_wf (t1 ∩ t2)).
-Proof.
-  intros Hwf1%SIs_true_elim Hwf2%SIs_true_elim.
-  apply SIs_true_intro. revert Hwf1 Hwf2.
-  revert t2; induction t1 as [[]|[]]; intros [[]|[] ??]; simpl; eauto.
-Qed.
-Lemma coPset_opp_wf t : SIs_true (coPset_wf (coPset_opp_raw t)).
-Proof. apply SIs_true_intro. induction t as [[]|[]]; simpl; eauto. Qed.
+  coPset_wf t1 → coPset_wf t2 → coPset_wf (t1 ∩ t2).
+Proof. revert t2; induction t1 as [[]|[]]; intros [[]|[] ??]; simpl; eauto. Qed.
+Lemma coPset_opp_wf t : coPset_wf (coPset_opp_raw t).
+Proof. induction t as [[]|[]]; simpl; eauto. Qed.
 Lemma coPset_elem_of_singleton p q : e_of p (coPset_singleton_raw q) ↔ p = q.
 Proof.
   split; [|by intros <-; induction p; simpl; rewrite ?coPset_elem_of_node].
@@ -161,40 +150,22 @@ Proof.
 Qed.
 
 (** * Packed together + set operations *)
-(** Add an underscore to [CoPset_] to avoid nameclash with Iris's
-[algebra.coPset.CoPset]. *)
-Record coPset := CoPset_ {
-  coPset_car : coPset_raw;
-  coPset_prf : SIs_true (coPset_wf coPset_car);
-}.
-
-Lemma coPset_eq (X1 X2 : coPset) : X1 = X2 ↔ coPset_car X1 = coPset_car X2.
-Proof.
-  split; [by intros ->|intros].
-  destruct X1 as [t1 ?], X2 as [t2 ?]; by simplify_eq/=.
-Qed.
-Global Instance coPset_eq_dec : EqDecision coPset := λ X1 X2,
-  match coPset_raw_eq_dec (coPset_car X1) (coPset_car X2) with
-  | left H => left (proj2 (coPset_eq X1 X2) H)
-  | right H => right (H ∘ proj1 (coPset_eq X1 X2))
-  end.
+Definition coPset := { t | coPset_wf t }.
 
 Global Instance coPset_singleton : Singleton positive coPset := λ p,
-  CoPset_ (coPset_singleton_raw p) (coPset_singleton_wf _).
-Global Instance coPset_elem_of : ElemOf positive coPset := λ p X,
-  e_of p (coPset_car X).
-Global Instance coPset_empty : Empty coPset := CoPset_ (coPLeaf false) (squash I).
-Global Instance coPset_top : Top coPset := CoPset_ (coPLeaf true) (squash I).
-Global Instance coPset_union : Union coPset :=
-  λ '(CoPset_ t1 Ht1) '(CoPset_ t2 Ht2),
-    CoPset_ (t1 ∪ t2) (coPset_union_wf _ _ Ht1 Ht2).
-Global Instance coPset_intersection : Intersection coPset :=
-  λ '(CoPset_ t1 Ht1) '(CoPset_ t2 Ht2),
-    CoPset_ (t1 ∩ t2) (coPset_intersection_wf _ _ Ht1 Ht2).
-Global Instance coPset_difference : Difference coPset :=
-  λ '(CoPset_ t1 Ht1) '(CoPset_ t2 Ht2),
-    CoPset_ (t1 ∩ coPset_opp_raw t2)
-           (coPset_intersection_wf _ _ Ht1 (coPset_opp_wf _)).
+  coPset_singleton_raw p ↾ coPset_singleton_wf _.
+Global Instance coPset_elem_of : ElemOf positive coPset := λ p X, e_of p (`X).
+Global Instance coPset_empty : Empty coPset := coPLeaf false ↾ I.
+Global Instance coPset_top : Top coPset := coPLeaf true ↾ I.
+Global Instance coPset_union : Union coPset := λ X Y,
+  let (t1,Ht1) := X in let (t2,Ht2) := Y in
+  (t1 ∪ t2) ↾ coPset_union_wf _ _ Ht1 Ht2.
+Global Instance coPset_intersection : Intersection coPset := λ X Y,
+  let (t1,Ht1) := X in let (t2,Ht2) := Y in
+  (t1 ∩ t2) ↾ coPset_intersection_wf _ _ Ht1 Ht2.
+Global Instance coPset_difference : Difference coPset := λ X Y,
+  let (t1,Ht1) := X in let (t2,Ht2) := Y in
+  (t1 ∩ coPset_opp_raw t2) ↾ coPset_intersection_wf _ _ Ht1 (coPset_opp_wf _).
 
 Global Instance coPset_top_set : TopSet positive coPset.
 Proof.
@@ -218,22 +189,22 @@ Global Hint Resolve coPset_top_subseteq : core.
 Global Instance coPset_leibniz : LeibnizEquiv coPset.
 Proof.
   intros X Y; rewrite set_equiv; intros HXY.
-  apply coPset_eq, coPset_wf_eq; [|apply SIs_true_elim, coPset_prf..].
+  apply (sig_eq_pi _), coPset_eq; try apply @proj2_sig.
   intros p; apply eq_bool_prop_intro, (HXY p).
 Qed.
+
 Global Instance coPset_elem_of_dec : RelDecision (∈@{coPset}).
 Proof. solve_decision. Defined.
 Global Instance coPset_equiv_dec : RelDecision (≡@{coPset}).
-Proof. refine (λ X Y, cast_if (decide (X = Y))); abstract (by fold_leibniz). Qed.
+Proof. refine (λ X Y, cast_if (decide (X = Y))); abstract (by fold_leibniz). Defined.
 Global Instance mapset_disjoint_dec : RelDecision (##@{coPset}).
 Proof.
-  refine (λ X Y, cast_if (decide (X ∩ Y = ∅)));
-   abstract (by rewrite disjoint_intersection_L).
+ refine (λ X Y, cast_if (decide (X ∩ Y = ∅)));
+  abstract (by rewrite disjoint_intersection_L).
 Defined.
 Global Instance mapset_subseteq_dec : RelDecision (⊆@{coPset}).
 Proof.
-  refine (λ X Y, cast_if (decide (X ∪ Y = Y)));
-    abstract (by rewrite subseteq_union_L).
+ refine (λ X Y, cast_if (decide (X ∪ Y = Y))); abstract (by rewrite subseteq_union_L).
 Defined.
 
 (** * Finite sets *)
@@ -244,7 +215,7 @@ Fixpoint coPset_finite (t : coPset_raw) : bool :=
 Lemma coPset_finite_node b l r :
   coPset_finite (coPNode' b l r) = coPset_finite l && coPset_finite r.
 Proof. by destruct b, l as [[]|], r as [[]|]. Qed.
-Lemma coPset_finite_spec X : set_finite X ↔ coPset_finite (coPset_car X).
+Lemma coPset_finite_spec X : set_finite X ↔ coPset_finite (`X).
 Proof.
   destruct X as [t Ht].
   unfold set_finite, elem_of at 1, coPset_elem_of; simpl; clear Ht; split.
@@ -263,8 +234,7 @@ Proof.
 Qed.
 Global Instance coPset_finite_dec (X : coPset) : Decision (set_finite X).
 Proof.
-  refine (cast_if (decide (coPset_finite (coPset_car X))));
-    by rewrite coPset_finite_spec.
+  refine (cast_if (decide (coPset_finite (`X)))); by rewrite coPset_finite_spec.
 Defined.
 
 (** * Pick element from infinite sets *)
@@ -282,8 +252,7 @@ Fixpoint coPpick_raw (t : coPset_raw) : option positive :=
      | Some i => Some (i~0) | None => (~1) <$> coPpick_raw r
      end
   end.
-Definition coPpick (X : coPset) : positive :=
-  default 1 (coPpick_raw (coPset_car X)).
+Definition coPpick (X : coPset) : positive := default 1 (coPpick_raw (`X)).
 
 Lemma coPpick_raw_elem_of t i : coPpick_raw t = Some i → e_of i t.
 Proof.
@@ -309,15 +278,10 @@ Fixpoint coPset_to_Pset_raw (t : coPset_raw) : Pmap_raw () :=
   | coPNode false l r => PNode' None (coPset_to_Pset_raw l) (coPset_to_Pset_raw r)
   | coPNode true l r => PNode (Some ()) (coPset_to_Pset_raw l) (coPset_to_Pset_raw r)
   end.
-Lemma coPset_to_Pset_wf t :
-  SIs_true (coPset_wf t) → SIs_true (Pmap_wf (coPset_to_Pset_raw t)).
-Proof.
-  intros Hwf%SIs_true_elim. apply SIs_true_intro.
-  induction t as [|[]]; simpl; eauto using PNode_wf.
-Qed.
+Lemma coPset_to_Pset_wf t : coPset_wf t → Pmap_wf (coPset_to_Pset_raw t).
+Proof. induction t as [|[]]; simpl; eauto using PNode_wf. Qed.
 Definition coPset_to_Pset (X : coPset) : Pset :=
-  let (t,Ht) := X in
-  Mapset (PMap (coPset_to_Pset_raw t) (coPset_to_Pset_wf _ Ht)).
+  let (t,Ht) := X in Mapset (PMap (coPset_to_Pset_raw t) (coPset_to_Pset_wf _ Ht)).
 Lemma elem_of_coPset_to_Pset X i : set_finite X → i ∈ coPset_to_Pset X ↔ i ∈ X.
 Proof.
   rewrite coPset_finite_spec; destruct X as [t Ht].
@@ -333,10 +297,8 @@ Fixpoint Pset_to_coPset_raw (t : Pmap_raw ()) : coPset_raw :=
   | PNode None l r => coPNode false (Pset_to_coPset_raw l) (Pset_to_coPset_raw r)
   | PNode (Some _) l r => coPNode true (Pset_to_coPset_raw l) (Pset_to_coPset_raw r)
   end.
-Lemma Pset_to_coPset_wf t :
-  SIs_true (Pmap_wf t) → SIs_true (coPset_wf (Pset_to_coPset_raw t)).
+Lemma Pset_to_coPset_wf t : Pmap_wf t → coPset_wf (Pset_to_coPset_raw t).
 Proof.
-  intros Hwf%SIs_true_elim. apply SIs_true_intro. revert Hwf.
   induction t as [|[] l IHl r IHr]; simpl; rewrite ?andb_True; auto.
   - intros [??]; destruct l as [|[]], r as [|[]]; simpl in *; auto.
   - destruct l as [|[]], r as [|[]]; simpl in *; rewrite ?andb_true_r;
@@ -348,8 +310,7 @@ Lemma Pset_to_coPset_raw_finite t : coPset_finite (Pset_to_coPset_raw t).
 Proof. induction t as [|[[]|]]; simpl; rewrite ?andb_True; auto. Qed.
 
 Definition Pset_to_coPset (X : Pset) : coPset :=
-  let 'Mapset (PMap t Ht) := X in
-  CoPset_ (Pset_to_coPset_raw t) (Pset_to_coPset_wf _ Ht).
+  let 'Mapset (PMap t Ht) := X in Pset_to_coPset_raw t ↾ Pset_to_coPset_wf _ Ht.
 Lemma elem_of_Pset_to_coPset X i : i ∈ Pset_to_coPset X ↔ i ∈ X.
 Proof. destruct X as [[t ?]]; apply elem_of_Pset_to_coPset_raw. Qed.
 Lemma Pset_to_coPset_finite X : set_finite (Pset_to_coPset X).
@@ -359,14 +320,13 @@ Qed.
 
 (** * Conversion to and from gsets of positives *)
 Lemma coPset_to_gset_wf (m : Pmap ()) : gmap_wf positive m.
-Proof. by apply squash. Qed.
+Proof. unfold gmap_wf. by rewrite bool_decide_spec. Qed.
 Definition coPset_to_gset (X : coPset) : gset positive :=
   let 'Mapset m := coPset_to_Pset X in
   Mapset (GMap m (coPset_to_gset_wf m)).
 
 Definition gset_to_coPset (X : gset positive) : coPset :=
-  let 'Mapset (GMap (PMap t Ht) _) := X in
-  CoPset_ (Pset_to_coPset_raw t) (Pset_to_coPset_wf _ Ht).
+  let 'Mapset (GMap (PMap t Ht) _) := X in Pset_to_coPset_raw t ↾ Pset_to_coPset_wf _ Ht.
 
 Lemma elem_of_coPset_to_gset X i : set_finite X → i ∈ coPset_to_gset X ↔ i ∈ X.
 Proof.
@@ -420,10 +380,10 @@ Fixpoint coPset_suffixes_raw (p : positive) : coPset_raw :=
   | p~0 => coPNode' false (coPset_suffixes_raw p) (coPLeaf false)
   | p~1 => coPNode' false (coPLeaf false) (coPset_suffixes_raw p)
   end.
-Lemma coPset_suffixes_wf p : SIs_true (coPset_wf (coPset_suffixes_raw p)).
-Proof. apply SIs_true_intro. induction p; simpl; eauto. Qed.
+Lemma coPset_suffixes_wf p : coPset_wf (coPset_suffixes_raw p).
+Proof. induction p; simpl; eauto. Qed.
 Definition coPset_suffixes (p : positive) : coPset :=
-  CoPset_ (coPset_suffixes_raw p) (coPset_suffixes_wf _).
+  coPset_suffixes_raw p ↾ coPset_suffixes_wf _.
 Lemma elem_coPset_suffixes p q : p ∈ coPset_suffixes q ↔ ∃ q', p = q' ++ q.
 Proof.
   unfold elem_of, coPset_elem_of; simpl; split.
@@ -451,14 +411,14 @@ Fixpoint coPset_r_raw (t : coPset_raw) : coPset_raw :=
   | coPNode b l r => coPNode' false (coPset_r_raw l) (coPset_r_raw r)
   end.
 
-Lemma coPset_l_wf t : SIs_true (coPset_wf (coPset_l_raw t)).
-Proof. apply SIs_true_intro. induction t as [[]|]; simpl; auto. Qed.
-Lemma coPset_r_wf t : SIs_true (coPset_wf (coPset_r_raw t)).
-Proof. apply SIs_true_intro.  induction t as [[]|]; simpl; auto. Qed.
+Lemma coPset_l_wf t : coPset_wf (coPset_l_raw t).
+Proof. induction t as [[]|]; simpl; auto. Qed.
+Lemma coPset_r_wf t : coPset_wf (coPset_r_raw t).
+Proof. induction t as [[]|]; simpl; auto. Qed.
 Definition coPset_l (X : coPset) : coPset :=
-  let (t,Ht) := X in CoPset_ (coPset_l_raw t) (coPset_l_wf _).
+  let (t,Ht) := X in coPset_l_raw t ↾ coPset_l_wf _.
 Definition coPset_r (X : coPset) : coPset :=
-  let (t,Ht) := X in CoPset_ (coPset_r_raw t) (coPset_r_wf _).
+  let (t,Ht) := X in coPset_r_raw t ↾ coPset_r_wf _.
 
 Lemma coPset_lr_disjoint X : coPset_l X ∩ coPset_r X = ∅.
 Proof.
