theories/pmap.v
@@ -126,36 +126,24 @@ Lemma PNode_lookup {A} o (l r : Pmap_raw A) i :
   PNode' o l r !! i = PNode o l r !! i.
 Proof. by destruct i, o, l, r. Qed.
 
-Local Lemma Psingleton_wf' {A} i (x : A) : Pmap_wf (Psingleton_raw i x).
+Lemma Psingleton_wf {A} i (x : A) : Pmap_wf (Psingleton_raw i x).
 Proof. induction i as [[]|[]|]; simpl; rewrite ?andb_true_r; auto. Qed.
-Local Lemma Ppartial_alter_wf {A} f i (t : Pmap_raw A) :
-  SIs_true (Pmap_wf t) → SIs_true (Pmap_wf (Ppartial_alter_raw f i t)).
+Lemma Ppartial_alter_wf {A} f i (t : Pmap_raw A) :
+  Pmap_wf t → Pmap_wf (Ppartial_alter_raw f i t).
 Proof.
-  intros Hwf%SIs_true_elim. apply SIs_true_intro. revert Hwf.
   revert i; induction t as [|o l IHl r IHr]; intros i ?; simpl.
-  - destruct (f None); auto using Psingleton_wf'.
+  - destruct (f None); auto using Psingleton_wf.
   - destruct i; simpl; eauto.
 Qed.
-Local Lemma Pfmap_wf {A B} (f : A → B) t :
-  SIs_true (Pmap_wf t) → SIs_true (Pmap_wf (Pfmap_raw f t)).
+Lemma Pfmap_wf {A B} (f : A → B) t : Pmap_wf t → Pmap_wf (Pfmap_raw f t).
 Proof.
-  intros Hwf%SIs_true_elim. apply SIs_true_intro. revert Hwf.
   induction t as [|[x|] [] ? [] ?]; simpl in *; rewrite ?andb_True; intuition.
 Qed.
-Local Lemma Pomap_wf' {A B} (f : A → option B) t :
-  Pmap_wf t → Pmap_wf (Pomap_raw f t).
+Lemma Pomap_wf {A B} (f : A → option B) t : Pmap_wf t → Pmap_wf (Pomap_raw f t).
 Proof. induction t; simpl; eauto. Qed.
-Local Lemma Pomap_wf {A B} (f : A → option B) t :
-  SIs_true (Pmap_wf t) → SIs_true (Pmap_wf (Pomap_raw f t)).
-Proof. intros. by apply SIs_true_intro, Pomap_wf', SIs_true_elim. Qed.
-Local Lemma Pmerge_wf {A B C} (f : option A → option B → option C) t1 t2 :
-  SIs_true (Pmap_wf t1) → SIs_true (Pmap_wf t2) →
-  SIs_true (Pmap_wf (Pmerge_raw f t1 t2)).
-Proof.
-  intros Hwf1%SIs_true_elim Hwf2%SIs_true_elim.
-  apply SIs_true_intro. revert Hwf1 Hwf2.
-  revert t2. induction t1; intros []; simpl; eauto using Pomap_wf'.
-Qed.
+Lemma Pmerge_wf {A B C} (f : option A → option B → option C) t1 t2 :
+  Pmap_wf t1 → Pmap_wf t2 → Pmap_wf (Pmerge_raw f t1 t2).
+Proof. revert t2. induction t1; intros []; simpl; eauto using Pomap_wf. Qed.
 
 Lemma Plookup_empty {A} i : (∅ : Pmap_raw A) !! i = None.
 Proof. by destruct i. Qed.
@@ -266,42 +254,38 @@ Proof.
 Qed.
 
 (** Packed version and instance of the finite map type class *)
-Record Pmap (A : Type) : Type :=
-  PMap { pmap_car : Pmap_raw A; pmap_prf : SIs_true (Pmap_wf pmap_car) }.
+Inductive Pmap (A : Type) : Type :=
+  PMap { pmap_car : Pmap_raw A; pmap_prf : Pmap_wf pmap_car }.
 Global Arguments PMap {_} _ _ : assert.
 Global Arguments pmap_car {_} _ : assert.
 Global Arguments pmap_prf {_} _ : assert.
-
 Lemma Pmap_eq {A} (m1 m2 : Pmap A) : m1 = m2 ↔ pmap_car m1 = pmap_car m2.
 Proof.
   split; [by intros ->|intros]; destruct m1 as [t1 ?], m2 as [t2 ?].
-  simplify_eq/=; f_equal.
+  simplify_eq/=; f_equal; apply proof_irrel.
 Qed.
 Global Instance Pmap_eq_dec `{EqDecision A} : EqDecision (Pmap A) := λ m1 m2,
   match Pmap_raw_eq_dec (pmap_car m1) (pmap_car m2) with
   | left H => left (proj2 (Pmap_eq m1 m2) H)
   | right H => right (H ∘ proj1 (Pmap_eq m1 m2))
   end.
-
-Global Instance Pempty {A} : Empty (Pmap A) := PMap ∅ (squash I).
+Global Instance Pempty {A} : Empty (Pmap A) := PMap ∅ I.
 Global Instance Plookup {A} : Lookup positive A (Pmap A) := λ i m, pmap_car m !! i.
-Global Instance Ppartial_alter {A} : PartialAlter positive A (Pmap A) :=
-  λ f i '(PMap t Ht),
-    PMap (partial_alter f i t) (Ppartial_alter_wf f i _ Ht).
-Global Instance Pfmap : FMap Pmap := λ A B f '(PMap t Ht),
-  PMap (f <$> t) (Pfmap_wf f _ Ht).
-Global Instance Pto_list {A} : FinMapToList positive A (Pmap A) := λ '(PMap t Ht),
-  Pto_list_raw 1 t [].
-Global Instance Pomap : OMap Pmap := λ A B f '(PMap t Ht),
-  PMap (omap f t) (Pomap_wf f _ Ht).
-Global Instance Pmerge : Merge Pmap := λ A B C f '(PMap t1 Ht1) '(PMap t2 Ht2),
-  PMap _ (Pmerge_wf f _ _ Ht1 Ht2).
+Global Instance Ppartial_alter {A} : PartialAlter positive A (Pmap A) := λ f i m,
+  let (t,Ht) := m in PMap (partial_alter f i t) (Ppartial_alter_wf f i _ Ht).
+Global Instance Pfmap : FMap Pmap := λ A B f m,
+  let (t,Ht) := m in PMap (f <$> t) (Pfmap_wf f _ Ht).
+Global Instance Pto_list {A} : FinMapToList positive A (Pmap A) := λ m,
+  let (t,Ht) := m in Pto_list_raw 1 t [].
+Global Instance Pomap : OMap Pmap := λ A B f m,
+  let (t,Ht) := m in PMap (omap f t) (Pomap_wf f _ Ht).
+Global Instance Pmerge : Merge Pmap := λ A B C f m1 m2,
+  let (t1,Ht1) := m1 in let (t2,Ht2) := m2 in PMap _ (Pmerge_wf f _ _ Ht1 Ht2).
 
 Global Instance Pmap_finmap : FinMap positive Pmap.
 Proof.
- split.
-  - intros ? [t1 ?] [t2 ?] ?.
-    apply Pmap_eq, Pmap_wf_eq; auto using SIs_true_elim.
+  split.
+  - by intros ? [t1 ?] [t2 ?] ?; apply Pmap_eq, Pmap_wf_eq.
   - by intros ? [].
   - intros ?? [??] ?. by apply Plookup_alter.
   - intros ?? [??] ??. by apply Plookup_alter_ne.
